SlowTest/DiffLogic-Test/VU_Dafny.dfy
@@ -1,0 +1,93 @@
+// VectorUpdate-seq.dfy
+
+function method Dec(a: int, b: int) : int
+lemma Props_dec_one (sum: int)
+    ensures forall j :: Dec(sum, j + 1) < Dec(sum, j)
+lemma Props_dec_lower_bound (sum: int, x: int)
+    requires x <= sum
+    ensures 0 <= Dec(sum, x)
+
+function method Div(a: int, b: int): (c: int)
+    requires b != 0
+    ensures a == 100 && b == 9 ==> c == 11
+    ensures a == 100 && b == 10 ==> c == 10
+    { a / b }
+
+function method Add(a: int, b: int): (c: int)
+    ensures a == 11 && b == 10 ==> c == 21
+    { assert 11 + 10 == 21;
+      assert a == 11 && b == 10 ==> a + b == 21; // failed
+      a + b }
+
+method VectorUpdate<A>(N: int, a : seq<A>, f : (int,A) ~> A) returns (a': seq<A>)
+  requires N == |a|
+  requires forall j :: 0 <= j < N ==> f.requires(j,a[j])
+  ensures |a| == |a'|
+  ensures forall j :: 0 <= j < N ==> a'[j] == f(j,a[j])
+{
+  var i := 0;
+  a' := a;
+  while i < N
+    invariant 0 <= i <= N
+    invariant |a| == |a'|
+    invariant forall j :: i <= j < N ==> f.requires(j,a[j])
+    invariant forall j :: 0 <= j < N ==> f.requires(j,a[j])
+    invariant forall j :: i <= j < N ==> a'[j] == a[j]
+    invariant forall j :: 0 <= j < i ==> a'[j] == f(j,a[j])
+    decreases Dec(N, i)
+  {
+    a' := a'[i := f(i,a[i])];
+    Props_dec_one (N);
+    Props_dec_lower_bound(N, i);
+    i := i + 1;
+  }
+}
+
+function method SeqInit<X> (len: int, func : int --> X) : (s: seq<X>)
+  requires len >= 0
+  requires forall i : int :: 0 <= i < len ==> func.requires(i)
+  ensures |s| == len
+  ensures forall i : int :: 0 <= i < len ==> s[i] == func(i)
+
+method Main()
+{
+  // v = [0, 0, 0, 0, 0, 0, 0, 0, 0, 0]
+  var v := SeqInit(10, _ => 0);
+  // v' = [0, 1, 2, 3, 4, 5, 6, 7, 8, 9]
+  var v' := VectorUpdate(10, v, (i,_) => i);
+  assert |v'| == |v|;
+  PrintSeq(v');
+  // v' = [1, 2, 3, 4, 5, 6, 7, 8, 9, 10]
+  v' := VectorUpdate(10, v', (_,x) => x + 1);
+  PrintSeq(v');
+  // v' = [100, 50, 33, 25, 20, 16, 14, 12, 11, 10]
+  v' := VectorUpdate(10, v', (_,x) requires x != 0 => Div(100, x));
+  PrintSeq(v');
+
+  // u = [0, 0, 0, 0, 0, 0, 0, 0, 0, 0]
+  var u := SeqInit(10, _ => 0);
+  // u' = [100, 50, 33, 25, 20, 16, 14, 12, 11, 10]
+  u := VectorUpdate(10, u, (i,_) requires 0 <= i < 10 => v'[i]);
+  PrintSeq(u);
+  
+  // z = [0, 0, 0, 0, 0, 0, 0, 0, 0]
+  var z := SeqInit(9, _ => 0);
+  // z' = [150, 83, 58, 45, 35, 30, 26, 23, 21]
+//   z := VectorUpdate(9, z, (i,_) requires 0 <= i < 9 => u[i] + u[i+1]);
+  z := VectorUpdate(9, z, (i,_) requires 0 <= i < 9 => Add(u[i], u[i+1]));
+  PrintSeq(z);
+  assert z[8] == 21;
+}
+
+method PrintSeq(a : seq<int>)
+{
+  // var i := 0;
+  // while i < |a| {
+  //   if i != 0 {
+	//   print ", ";
+	// }
+  //   print a[i];
+  //   i := i + 1;
+  // }
+  // print "\n";
+}
